import 2017 version of L3_Lib from Cambridge

L3_Lib/L3_Lib.thy
@@ -1,49 +1,35 @@
 (*  Title: L3_Lib.thy
-    Author: Anthony Fox, University of Cambridge
+    Original author: Anthony Fox, University of Cambridge
+    Contributions by: Kyndylan Nienhuis <kyndylan@mutlus.nl>
 
 L3 operations.
 *)
+
 theory L3_Lib
-imports "HOL-Word.Word"
-        "HOL-Library.Code_Target_Numeral"
-        "HOL-Library.Code_Char"
-        "HOL-Library.Monad_Syntax"
+imports "$ISABELLE_HOME/src/HOL/Word/Word"
+        "$ISABELLE_HOME/src/HOL/Library/Code_Target_Numeral"
+        "$ISABELLE_HOME/src/HOL/Library/Code_Char"
 begin
-
-(* enable printing for do notation *)
-translations
-  "_do_block (_do_cons (_do_bind p t) (_do_final e))"
-    <= "CONST bind t (\<lambda>p. e)"
-
-(* avoid syntax clash with shift-right operation *)
-no_syntax
-  "_thenM" :: "['a, 'b] \<Rightarrow> 'c" (infixr ">>" 54)
-
 
 (* basic state Monad *)
 
 definition "return = Pair"
-declare return_def [simp add]
 
-fun bind :: "('state \<Rightarrow> ('a \<times> 'state)) \<Rightarrow>
-             ('a \<Rightarrow> 'state \<Rightarrow> ('b \<times> 'state)) \<Rightarrow>
-             ('state \<Rightarrow> ('b \<times> 'state))" where
+definition bind :: "('state \<Rightarrow> ('a \<times> 'state)) \<Rightarrow>
+                    ('a \<Rightarrow> 'state \<Rightarrow> ('b \<times> 'state)) \<Rightarrow>
+                    ('state \<Rightarrow> ('b \<times> 'state))" where
   "bind f g = (\<lambda>s. let (a, s') = f s in g a s')"
 
-(* use do syntax for this state monad *)
-adhoc_overloading
-  Monad_Syntax.bind bind 
-
-fun read_state :: "('state \<Rightarrow> 'a) \<Rightarrow> 'state \<Rightarrow> 'a \<times> 'state" where
+definition read_state :: "('state \<Rightarrow> 'a) \<Rightarrow> 'state \<Rightarrow> 'a \<times> 'state" where
   "read_state f = (\<lambda>s. (f s, s))"
 
-fun update_state :: "('state \<Rightarrow> 'state) \<Rightarrow> 'state \<Rightarrow> unit \<times> 'state" where
+definition update_state :: "('state \<Rightarrow> 'state) \<Rightarrow> 'state \<Rightarrow> unit \<times> 'state" where
   "update_state f = (\<lambda>s. ((), f s))"
 
-fun extend_state :: "'b \<Rightarrow> ('b \<times> 'state \<Rightarrow> 'a \<times> 'b \<times> 'state) \<Rightarrow> 'state \<Rightarrow> 'a \<times> 'state" where
+definition extend_state :: "'b \<Rightarrow> ('b \<times> 'state \<Rightarrow> 'a \<times> 'b \<times> 'state) \<Rightarrow> 'state \<Rightarrow> 'a \<times> 'state" where
   "extend_state v f = (\<lambda>s. let (a, s') = f (v, s) in (a, snd s'))"
 
-fun trim_state :: "('state \<Rightarrow> 'a \<times> 'state) \<Rightarrow> 'b \<times> 'state \<Rightarrow> 'a \<times> 'b \<times> 'state" where
+definition trim_state :: "('state \<Rightarrow> 'a \<times> 'state) \<Rightarrow> 'b \<times> 'state \<Rightarrow> 'a \<times> 'b \<times> 'state" where
   "trim_state f = (\<lambda>(s1, s2). let (a, s') = f s2 in (a, s1, s'))"
 
 fun foreach_loop :: "'a list \<times> ('a \<Rightarrow> 'state \<Rightarrow> unit \<times> 'state) \<Rightarrow> 'state \<Rightarrow> unit \<times> 'state" where
@@ -59,40 +45,119 @@ function for_loop :: "nat \<times> nat \<times> (nat \<Rightarrow> 'state \<Righ
   by auto
   termination by (relation "measure (\<lambda>(i, j, _). if i < j then j - i else i - j)") auto
 
+(* Because there are no constraints on i, j and a on the left-hand side of the definition, every
+occurrence of for_loop can be simplified by for_loop.simps, and since the definition is recursive
+the simplifier might diverge. For this reason we remove for_loop.simps from the simp set. *)
+
+declare for_loop.simps [simp del]
+
+(* Monad laws *)
+
+lemma bind_left_identity [simp]:
+  shows "bind (return a) f = f a"
+unfolding return_def bind_def
+by auto
+
+lemma bind_right_identity [simp]:
+  shows "bind m return = m"
+unfolding return_def bind_def
+by auto
+
+lemma bind_associativity:
+  shows "bind (bind m f) g = bind m (\<lambda>a. bind (f a) g)" 
+        (is "?l = ?r")
+proof
+  fix s
+  show "?l s = ?r s"
+    unfolding return_def bind_def 
+    by (cases "m s") auto
+qed
+
+(* Projections *)
+
+lemma project_return [simp]:
+  shows "fst (return a s) = a"
+    and "snd (return a s) = s"
+unfolding return_def
+by auto
+
+lemma project_read_state [simp]:
+  shows "fst (read_state f s) = f s"
+    and "snd (read_state f s) = s"
+unfolding read_state_def
+by auto
+
+lemma project_update_state [simp]:
+  shows "fst (update_state f s) = ()"
+    and "snd (update_state f s) = f s"
+unfolding update_state_def
+by auto
+
+(* Other monad simplifications *)
+
+lemma read_state_constant [simp]:
+  shows "read_state (\<lambda>s. a) = return a" 
+unfolding read_state_def return_def
+..
+
+lemma update_state_id [simp]:
+  shows "update_state (\<lambda>s. s) = return ()" 
+unfolding update_state_def return_def
+..
+
+lemma foreach_loop_return [simp]:
+  shows "foreach_loop (l, \<lambda>_. return a) = return ()"
+by (induct l) simp_all
+
+lemma extend_state_return [simp]:
+  shows "extend_state v (return a) = return a"
+unfolding extend_state_def return_def
+by simp
+
+lemma extend_state_trim_state [simp]:
+  shows "extend_state v (trim_state m) = m" 
+        (is "?l = ?r")
+proof
+  fix s
+  show "?l s = ?r s"
+    unfolding extend_state_def trim_state_def
+    by (cases "m s") auto
+qed
+
 (* extra character operations *)
 
-fun Ord :: "char \<Rightarrow> nat" where
-   "Ord (Char nh nl) = nat_of_nibble nh * 16 + nat_of_nibble nl"
+definition Ord :: "char \<Rightarrow> nat" where
+   "Ord = nat_of_char" 
 
-fun Chr :: "nat \<Rightarrow> char" where
-   "Chr n = Char (nibble_of_nat (n div 16)) (nibble_of_nat n)"
+definition Chr :: "nat \<Rightarrow> char" where
+   "Chr = char_of_nat"
 
-fun is_lower :: "char \<Rightarrow> bool" where
+definition is_lower :: "char \<Rightarrow> bool" where
    "is_lower c = (Ord (CHR ''a'') \<le> Ord c \<and> Ord c \<le> Ord (CHR ''z''))"
 
-fun is_upper :: "char \<Rightarrow> bool" where
+definition is_upper :: "char \<Rightarrow> bool" where
    "is_upper c = (Ord (CHR ''A'') \<le> Ord c \<and> Ord c \<le> Ord (CHR ''Z''))"
 
-fun is_space :: "char \<Rightarrow> bool" where
+definition is_space :: "char \<Rightarrow> bool" where
    "is_space c = (Ord (CHR '' '') = Ord c \<or> 9 \<le> Ord c \<and> Ord c \<le> 13)"
 
-fun is_digit :: "char \<Rightarrow> bool" where
+definition is_digit :: "char \<Rightarrow> bool" where
    "is_digit c = (Ord (CHR ''0'') \<le> Ord c \<and> Ord c \<le> Ord (CHR ''9''))"
 
-fun is_hex_digit :: "char \<Rightarrow> bool" where
+definition is_hex_digit :: "char \<Rightarrow> bool" where
    "is_hex_digit c = (is_digit c \<or> Ord (CHR ''a'') \<le> Ord c \<and> Ord c \<le> Ord (CHR ''f'') \<or>
                                    Ord (CHR ''A'') \<le> Ord c \<and> Ord c \<le> Ord (CHR ''F''))"
 
-fun is_alpha :: "char \<Rightarrow> bool" where
+definition is_alpha :: "char \<Rightarrow> bool" where
    "is_alpha c = (is_lower c \<or> is_upper c)"
 
-fun is_alpha_num :: "char \<Rightarrow> bool" where
+definition is_alpha_num :: "char \<Rightarrow> bool" where
    "is_alpha_num c = (is_alpha c \<or> is_digit c)"
 
-fun to_lower :: "char \<Rightarrow> char" where
+definition to_lower :: "char \<Rightarrow> char" where
    "to_lower c = (if is_upper c then Chr (Ord c + 32) else c)"
 
-fun to_upper :: "char \<Rightarrow> char" where
+definition to_upper :: "char \<Rightarrow> char" where
    "to_upper c = (if is_lower c then Chr (Ord c - 32) else c)"
 
 (* numeric strings *)
@@ -105,7 +170,13 @@ fun nat_to_list :: "nat \<Rightarrow> nat \<Rightarrow> nat list" where
   "nat_to_list base n =
    (if n < base \<or> base < 2 then [n mod base] else n mod base # nat_to_list base (n div base))"
 
-fun hex :: "nat \<Rightarrow> char" where
+(* Because there are no constraints on n on the left-hand side of the definition, every occurrence
+of nat_to_list can be simplified by nat_to_list.simps, and since the definition is recursive the
+simplifier might diverge. For this reason we remove nat_to_list.simps from the simp set. *)
+
+declare nat_to_list.simps [simp del]
+
+definition hex :: "nat \<Rightarrow> char" where
   "hex n = (if n = 0 then CHR ''0''
             else if n = 1 then CHR ''1''
             else if n = 2 then CHR ''2''
@@ -124,7 +195,7 @@ fun hex :: "nat \<Rightarrow> char" where
             else if n = 15 then CHR ''F''
             else undefined)"
 
-fun unhex :: "char \<Rightarrow> nat" where
+definition unhex :: "char \<Rightarrow> nat" where
   "unhex c = (if c = CHR ''0'' then 0
               else if c = CHR ''1'' then 1
               else if c = CHR ''2'' then 2
@@ -143,10 +214,10 @@ fun unhex :: "char \<Rightarrow> nat" where
               else if c = CHR ''f'' \<or> c = CHR ''F'' then 15
               else undefined)"
 
-fun string_to_nat :: "nat \<Rightarrow> string \<Rightarrow> nat" where
+definition string_to_nat :: "nat \<Rightarrow> string \<Rightarrow> nat" where
   "string_to_nat base s = list_to_nat base (map unhex (rev s))"
 
-fun nat_to_string :: "nat \<Rightarrow> nat \<Rightarrow> string" where
+definition nat_to_string :: "nat \<Rightarrow> nat \<Rightarrow> string" where
   "nat_to_string base n = rev (map hex (nat_to_list base n))"
 
 definition "bin_string_to_nat \<equiv> string_to_nat 2"
@@ -156,62 +227,127 @@ definition "nat_to_dec_string \<equiv> nat_to_string 10"
 definition "hex_string_to_nat \<equiv> string_to_nat 16"
 definition "nat_to_hex_string \<equiv> nat_to_string 16"
 
-fun nat_from_bin_string :: "string \<Rightarrow> nat option" where
+definition nat_from_bin_string :: "string \<Rightarrow> nat option" where
   "nat_from_bin_string s =
    (if s \<noteq> '''' \<and> list_all (\<lambda>c. c = CHR ''0'' \<or> c = CHR ''1'') s then
       Some (bin_string_to_nat s)
     else None)"
 
-fun nat_from_dec_string :: "string \<Rightarrow> nat option" where
+definition nat_from_dec_string :: "string \<Rightarrow> nat option" where
   "nat_from_dec_string s =
    (if s \<noteq> '''' \<and> list_all is_digit s then Some (dec_string_to_nat s) else None)"
 
-fun nat_from_hex_string :: "string \<Rightarrow> nat option" where
+definition nat_from_hex_string :: "string \<Rightarrow> nat option" where
   "nat_from_hex_string s =
    (if s \<noteq> '''' \<and> list_all is_hex_digit s then Some (hex_string_to_nat s) else None)"
 
-fun dec_string_to_int :: "string \<Rightarrow> int" where
-  "dec_string_to_int (CHR ''-'' # r) = -int (dec_string_to_nat r)" |
-  "dec_string_to_int (CHR ''~'' # r) = -int (dec_string_to_nat r)" |
-  "dec_string_to_int r = int (dec_string_to_nat r)"
+definition dec_string_to_int :: "string \<Rightarrow> int" where
+  "dec_string_to_int r = 
+   (case r of []    \<Rightarrow> 0 |
+              h # t \<Rightarrow> (if h = CHR ''-'' \<or> h = CHR ''~'' 
+                        then -int (dec_string_to_nat t)
+                        else  int (dec_string_to_nat r)))"
 
-fun int_to_dec_string :: "int \<Rightarrow> string" where
+definition int_to_dec_string :: "int \<Rightarrow> string" where
   "int_to_dec_string i =
    (if i < 0 then CHR ''~'' # nat_to_dec_string (nat (-i)) else nat_to_dec_string (nat i))"
 
-fun string_to_bool :: "string \<Rightarrow> bool" where
+definition string_to_bool :: "string \<Rightarrow> bool" where
   "string_to_bool s = (if s = ''true'' then True
                        else if s = ''false'' then False
                        else undefined)"
 
-fun string_to_char :: "string \<Rightarrow> char" where
-  "string_to_char [c] = c" |
-  "string_to_char _ = undefined"
+definition string_to_char :: "string \<Rightarrow> char" where
+  "string_to_char s = (case s of [c] \<Rightarrow> c | _ \<Rightarrow> undefined)"
 
 (* extra Nat operation *)
 
 fun log2 :: "nat \<Rightarrow> nat" where
   "log2 n = (if n = 0 then undefined else if n = 1 then 0 else Suc (log2 (n div 2)))"
 
+(* Because there are no constraints on n on the left-hand side of the definition, every occurrence
+of log2 can be simplified by log2.simps, and since the definition is recursive the simplifier might
+diverge. For this reason we remove log2.simps from the simp set. *)
+
+declare log2.simps [simp del]
+
+lemma log2_bounds:
+  assumes "n \<noteq> 0"
+  shows   "2 ^ (log2 n) \<le> n"
+    and   "n < 2 ^ (Suc (log2 n))"
+proof -
+  -- "The induction works better if we prove one goal instead of two goals"
+  have "2 ^ (log2 n) \<le> n \<and> n < 2 ^ (Suc (log2 n))"
+    using assms
+    proof (induct "log2 n" arbitrary: n)
+      case 0
+      hence "n = 1" 
+        by (simp add: log2.simps) (meson nat.simps(3))
+      thus ?case by (simp add: log2.simps)
+    next
+      case (Suc k)
+      show ?case
+        proof (cases "n = 1")
+          case True
+          thus ?thesis by (simp add: log2.simps)
+        next
+          case False
+          hence "1 < n" using Suc(3) by simp
+          hence "(n div 2) \<noteq> 0" by auto
+          have log2: "log2 n = Suc (log2 (n div 2))"
+            using `1 < n` by (simp add: log2.simps)
+          hence "k = log2 (n div 2)" using Suc(2) by simp
+          note Suc(1)[OF this `(n div 2) \<noteq> 0`]
+          thus ?thesis
+            using log2 by auto
+        qed
+    qed
+  thus "2 ^ (log2 n) \<le> n" "n < 2 ^ (Suc (log2 n))" by auto
+qed
+
+lemma log2_unat_bounds:
+  fixes x :: "('a :: len) word"
+  assumes "x \<noteq> 0"
+  shows "log2 (unat x) < len_of TYPE('a)"
+proof -
+  have "unat x \<noteq> 0" 
+    using assms 
+    by (simp add: unat_eq_zero)
+  have "unat x < 2 ^ len_of TYPE('a)"
+    by simp
+  note le_less_trans[OF log2_bounds(1)[OF `unat x \<noteq> 0`] this]
+  thus ?thesis by auto
+qed
+
 (* extra int operations *)
 
-fun quot :: "int \<Rightarrow> int \<Rightarrow> int" (infixl "quot" 70) where
+definition quot :: "int \<Rightarrow> int \<Rightarrow> int" (infixl "quot" 70) where
   "i quot j = (if j = 0 then undefined
                else if 0 < j then if 0 \<le> i then i div j else -(-i div j)
                else if 0 \<le> i then -(i div -j)
                else -i div -j)"
 
-fun rem :: "int \<Rightarrow> int \<Rightarrow> int" (infixl "rem" 70) where
+definition rem :: "int \<Rightarrow> int \<Rightarrow> int" (infixl "rem" 70) where
   "i rem j = (if j = 0 then undefined else i - i quot j * j)"
 
-fun quot_rem :: "int * int \<Rightarrow> int * int" where
-  "quot_rem (i, j) = (i div j, i rem j)"
+definition quot_rem :: "int * int \<Rightarrow> int * int" where
+  "quot_rem p = (case p of (i, j) \<Rightarrow> (i div j, i rem j))"
 
 (* extra option operations *)
 
-fun is_some :: "'a option \<Rightarrow> bool" where
-  "is_some (Some _) = True" |
-  "is_some _ = False"
+definition is_some :: "'a option \<Rightarrow> bool" where
+  "is_some x = (case x of Some _ \<Rightarrow> True | _ \<Rightarrow> False)"
+
+lemma is_some_alt:
+  shows "is_some x = (x \<noteq> None)"
+unfolding is_some_def 
+using option.disc_eq_case(2) 
+by auto
+
+lemma is_some_simps [simp]:
+  shows "\<not> (is_some None)"
+    and "is_some (Some x)"
+unfolding is_some_def by simp_all
 
 (* extra list operations *)
 
@@ -219,13 +355,13 @@ fun splitl :: "('a \<Rightarrow> bool) \<Rightarrow> 'a list \<Rightarrow> 'a li
   "splitl _ [] = ([], [])" |
   "splitl P (h # t) = (if P h then let (l, r) = splitl P t in (h # l, r) else ([], h # t))"
 
-fun splitr :: "('a \<Rightarrow> bool) \<Rightarrow> 'a list \<Rightarrow> 'a list \<times> 'a list" where
+definition splitr :: "('a \<Rightarrow> bool) \<Rightarrow> 'a list \<Rightarrow> 'a list \<times> 'a list" where
   "splitr P x = (let (l, r) = splitl P (rev x) in (rev r, rev l))"
 
-fun pad_left :: "'a \<Rightarrow> nat \<Rightarrow> 'a list \<Rightarrow> 'a list" where
+definition pad_left :: "'a \<Rightarrow> nat \<Rightarrow> 'a list \<Rightarrow> 'a list" where
   "pad_left c n s = replicate (n - length s) c @ s"
 
-fun pad_right :: "'a \<Rightarrow> nat \<Rightarrow> 'a list \<Rightarrow> 'a list" where
+definition pad_right :: "'a \<Rightarrow> nat \<Rightarrow> 'a list \<Rightarrow> 'a list" where
   "pad_right c n s = s @ replicate (n - length s) c"
 
 fun index_find :: "nat \<Rightarrow> 'a \<times> 'a list \<Rightarrow> nat option" where
@@ -233,23 +369,50 @@ fun index_find :: "nat \<Rightarrow> 'a \<times> 'a list \<Rightarrow> nat optio
   "index_find i (v, h # t) = (if v = h then Some i else index_find (Suc i) (v, t))"
 
 definition "index_of = index_find 0"
-declare index_of_def [simp add]
 
-fun remove :: "'a list * 'a list \<Rightarrow> 'a list" where
-  "remove (l1, l2) = filter (\<lambda>x. x \<notin> set l1) l2"
+definition remove :: "'a list * 'a list \<Rightarrow> 'a list" where
+  "remove p = (case p of (l1, l2) \<Rightarrow> filter (\<lambda>x. x \<notin> set l1) l2)"
 
-fun remove_except :: "'a list * 'a list \<Rightarrow> 'a list" where
-  "remove_except (l1, l2) = filter (\<lambda>x. x \<in> set l1) l2"
+definition remove_except :: "'a list * 'a list \<Rightarrow> 'a list" where
+  "remove_except p = (case p of (l1, l2) \<Rightarrow> filter (\<lambda>x. x \<in> set l1) l2)"
 
 fun remove_duplicates :: "'a list \<Rightarrow> 'a list" where
   "remove_duplicates [] = []" |
   "remove_duplicates (h # t) = (if h \<in> set t then remove_duplicates t else h # remove_duplicates t)"
 
-(* extra string operations *)
+lemma splitl_length:
+  shows "length (fst (splitl P l)) + length (snd (splitl P l)) = length l"
+by (induct l, auto simp add: case_prod_beta)
 
-lemma splitl_length [simp]:
+lemma splitl_fst_length [simp]:
+  shows "length (fst (splitl P x)) \<le> length x"
+using splitl_length 
+by (metis order_refl trans_le_add1)
+
+lemma splitl_snd_length [simp]:
   shows "length (snd (splitl P x)) \<le> length x"
-  by (induct x, auto simp add: case_prod_beta)
+using splitl_length 
+by (metis order_refl trans_le_add2)
+
+lemma pad_left_length [simp]:
+  shows "length (pad_left e n l) = max (length l) n"
+unfolding pad_left_def
+by auto 
+
+lemma pad_right_length [simp]:
+  shows "length (pad_right e n l) = max (length l) n"
+unfolding pad_right_def
+by auto
+
+lemma pad_left_nth:
+  shows "pad_left e n l ! m = 
+         (if m < n - List.length l 
+          then e 
+          else l ! (m - (n - List.length l)))"
+unfolding pad_left_def nth_append
+by simp
+
+(* extra string operations *)
 
 lemma fields_termination_lem [simp]:
   assumes "a \<noteq> []" and "length a \<le> length c"
@@ -284,16 +447,16 @@ function (sequential) fields :: "(char \<Rightarrow> bool) \<Rightarrow> string 
 
 (* bit-string operations - extends Bool_List_Representation.thy *)
 
-fun nat_to_bitstring :: "nat \<Rightarrow> bool list" where
-  "nat_to_bitstring 0 = [False]" |
-  "nat_to_bitstring n = bin_to_bl (log2 n + 1) (int n)"
+definition nat_to_bitstring :: "nat \<Rightarrow> bool list" where
+  "nat_to_bitstring n = 
+   (if n = 0 then [False] else bin_to_bl (log2 n + 1) (int n))"
 
 definition "bitstring_to_nat = nat o bl_to_bin"
 
-fun fixwidth :: "nat \<Rightarrow> bool list \<Rightarrow> bool list" where
+definition fixwidth :: "nat \<Rightarrow> bool list \<Rightarrow> bool list" where
   "fixwidth n v = (let l = length v in if l < n then pad_left False n v else drop (l - n) v)"
 
-fun bitwise :: "(bool \<Rightarrow> bool \<Rightarrow> bool) \<Rightarrow> bool list \<Rightarrow> bool list \<Rightarrow> bool list" where
+definition bitwise :: "(bool \<Rightarrow> bool \<Rightarrow> bool) \<Rightarrow> bool list \<Rightarrow> bool list \<Rightarrow> bool list" where
   "bitwise f v1 v2 =
    (let m = max (length v1) (length v2) in map (case_prod f) (zip (fixwidth m v1) (fixwidth m v2)))"
 
@@ -301,62 +464,90 @@ definition "bor  = bitwise (op \<or>)"
 definition "band = bitwise (op \<and>)"
 definition "bxor = bitwise (op \<noteq>)"
 
-fun bitstring_shiftl :: "bool list \<Rightarrow> nat \<Rightarrow> bool list" where
+definition bitstring_shiftl :: "bool list \<Rightarrow> nat \<Rightarrow> bool list" where
   "bitstring_shiftl v m = pad_right False (length v + m) v"
 
-fun bitstring_shiftr :: "bool list \<Rightarrow> nat \<Rightarrow> bool list" where
+definition bitstring_shiftr :: "bool list \<Rightarrow> nat \<Rightarrow> bool list" where
   "bitstring_shiftr v m = take (length v - m) v"
 
-fun bitstring_field :: "nat \<Rightarrow> nat \<Rightarrow> bool list \<Rightarrow> bool list" where
+definition bitstring_field :: "nat \<Rightarrow> nat \<Rightarrow> bool list \<Rightarrow> bool list" where
   "bitstring_field h l v = fixwidth (Suc h - l) (bitstring_shiftr v l)"
 
-fun bitstring_rotate :: "bool list \<Rightarrow> nat \<Rightarrow> bool list" where
+definition bitstring_rotate :: "bool list \<Rightarrow> nat \<Rightarrow> bool list" where
   "bitstring_rotate v m =
    (let l = length v in
     let x = m mod l in
       if l = 0 \<or> x = 0 then v else bitstring_field (x - 1) 0 v @ bitstring_field (l - 1) x v)"
 
-fun bitstring_test_bit :: "bool list \<Rightarrow> nat \<Rightarrow> bool" where
+definition bitstring_test_bit :: "bool list \<Rightarrow> nat \<Rightarrow> bool" where
   "bitstring_test_bit v n = (bitstring_field n n v = [True])"
 
-fun bitstring_modify ::  "(nat \<times> bool \<Rightarrow> bool) \<times> bool list \<Rightarrow> bool list" where
-  "bitstring_modify (f, l) = map f (zip (rev (upt 0 (length l))) l)"
+definition bitstring_modify ::  "(nat \<times> bool \<Rightarrow> bool) \<times> bool list \<Rightarrow> bool list" where
+  "bitstring_modify p = (case p of (f, l) \<Rightarrow> map f (zip (rev (upt 0 (length l))) l))"
 
-fun bitstring_field_insert :: "nat \<Rightarrow> nat \<Rightarrow> bool list \<Rightarrow> bool list \<Rightarrow> bool list" where
+definition bitstring_field_insert :: "nat \<Rightarrow> nat \<Rightarrow> bool list \<Rightarrow> bool list \<Rightarrow> bool list" where
   "bitstring_field_insert h l v1 v2 =
    bitstring_modify (\<lambda>(i, b). if l \<le> i \<and> i \<le> h then bitstring_test_bit v1 (i - l) else b, v2)"
 
+lemma nat_to_bitstring_zero [simp]:
+  shows "nat_to_bitstring 0 = [False]"
+unfolding nat_to_bitstring_def by simp
+
+(* We do not add the following rule to the simp set, because n occurs twice at the right hand side,
+and therefore the state might not become simpler when applying this rule. *)
+
+lemma nat_to_bitstring_length:
+  shows "length (nat_to_bitstring n) = (if n = 0 then 1 else log2 n + 1)"
+unfolding nat_to_bitstring_def
+by (simp del: bin_to_bl_def)
+
+lemma fixwidth_length [simp]:
+  shows "length (fixwidth n l) = n"
+unfolding fixwidth_def Let_def
+by auto
+
+lemma bitwise_length [simp]:
+  shows "length (bitwise f v1 v2) = max (length v1) (length v2)"
+unfolding bitwise_def Let_def
+by auto
+
 (* extra word operations *)
 
-fun unsigned_min :: "'a::len word \<times> 'a::len word \<Rightarrow> 'a::len word" where
-  "unsigned_min (w1, w2) = (if w1 \<le> w2 then w1 else w2)"
+definition unsigned_min :: "'a::len word \<times> 'a::len word \<Rightarrow> 'a::len word" where
+  "unsigned_min p = (case p of (w1, w2) \<Rightarrow> (if w1 \<le> w2 then w1 else w2))"
 
-fun unsigned_max :: "'a::len word \<times> 'a::len word \<Rightarrow> 'a::len word" where
-  "unsigned_max (w1, w2) = (if w1 \<le> w2 then w2 else w1)"
+definition unsigned_max :: "'a::len word \<times> 'a::len word \<Rightarrow> 'a::len word" where
+  "unsigned_max p = (case p of (w1, w2) \<Rightarrow> (if w1 \<le> w2 then w2 else w1))"
 
-fun word_log2 :: "'a::len word \<Rightarrow> 'a::len word" where
+definition word_log2 :: "'a::len word \<Rightarrow> 'a::len word" where
   "word_log2 w = of_nat (log2 (unat w))"
 
-fun word_quot :: "'a::len word \<Rightarrow> 'a::len word \<Rightarrow> 'a::len word" where
+definition word_quot :: "'a::len word \<Rightarrow> 'a::len word \<Rightarrow> 'a::len word" where
   "word_quot i j = of_int (sint i quot sint j)"
-
-fun word_rem :: "'a::len word \<Rightarrow> 'a::len word \<Rightarrow> 'a::len word" where
+  
+definition word_rem :: "'a::len word \<Rightarrow> 'a::len word \<Rightarrow> 'a::len word" where
   "word_rem i j = of_int (sint i rem sint j)"
 
-fun word_modify :: "(nat \<times> bool \<Rightarrow> bool) \<times> 'a::len word \<Rightarrow> 'a::len word" where
-  "word_modify (f, w) = of_bl (bitstring_modify (f, to_bl w))"
+definition word_sdiv :: "'a::len word \<Rightarrow> 'a::len word \<Rightarrow> 'a::len word" where
+  "word_sdiv i j = of_int (sint i div sint j)"
+  
+definition word_smod :: "'a::len word \<Rightarrow> 'a::len word \<Rightarrow> 'a::len word" where
+  "word_smod i j = of_int (sint i mod sint j)"
+  
+definition word_modify :: "(nat \<times> bool \<Rightarrow> bool) \<times> 'a::len word \<Rightarrow> 'a::len word" where
+  "word_modify p = (case p of (f, w) \<Rightarrow> of_bl (bitstring_modify (f, to_bl w)))"
 
-fun word_bit_field_insert :: "nat \<Rightarrow> nat \<Rightarrow> 'a::len word \<Rightarrow> 'b::len word \<Rightarrow> 'b::len word" where
+definition word_bit_field_insert :: "nat \<Rightarrow> nat \<Rightarrow> 'a::len word \<Rightarrow> 'b::len word \<Rightarrow> 'b::len word" where
   "word_bit_field_insert h l w1 w2 =
    word_modify (\<lambda>(i, b). if l \<le> i \<and> i \<le> h then test_bit w1 (i - l) else b, w2)"
 
-fun word_bits :: "nat \<Rightarrow> nat \<Rightarrow> 'a::len word \<Rightarrow> 'a::len word" where
+definition word_bits :: "nat \<Rightarrow> nat \<Rightarrow> 'a::len word \<Rightarrow> 'a::len word" where
   "word_bits h l w = (w >> l) AND mask (Suc h - l)"
 
-fun word_extract :: "nat \<Rightarrow> nat \<Rightarrow> 'a::len word \<Rightarrow> 'b::len word" where
+definition word_extract :: "nat \<Rightarrow> nat \<Rightarrow> 'a::len word \<Rightarrow> 'b::len word" where
   "word_extract h l w = ucast (word_bits h l w)"
 
-fun word_replicate :: "nat \<Rightarrow> 'a::len word \<Rightarrow> 'b::len word" where
+definition word_replicate :: "nat \<Rightarrow> 'a::len word \<Rightarrow> 'b::len word" where
   "word_replicate n a = word_rcat (replicate n a)"
 
 (* floating-point stubs *)
@@ -366,62 +557,97 @@ datatype ieee_rounding =
 
 datatype ieee_compare = LT | EQ | GT | UN
 
+record ieee_flags = 
+  DivideByZero :: bool
+  InvalidOp :: bool
+  Overflow :: bool
+  Precision :: bool
+  Underflow :: bool
+  
 consts
   fp32_abs :: "32 word \<Rightarrow> 32 word"
-  fp32_abs1985 :: "32 word \<Rightarrow> 32 word"
   fp32_add :: "ieee_rounding \<Rightarrow> 32 word \<Rightarrow> 32 word \<Rightarrow> 32 word"
+  fp32_add_with_flags :: "ieee_rounding \<Rightarrow> 32 word \<Rightarrow> 32 word \<Rightarrow> ieee_flags \<times> 32 word"
   fp32_compare :: "32 word \<Rightarrow> 32 word \<Rightarrow> ieee_compare"
   fp32_div :: "ieee_rounding \<Rightarrow> 32 word \<Rightarrow> 32 word \<Rightarrow> 32 word"
+  fp32_div_with_flags :: "ieee_rounding \<Rightarrow> 32 word \<Rightarrow> 32 word \<Rightarrow> ieee_flags \<times> 32 word"
   fp32_equal :: "32 word \<Rightarrow> 32 word \<Rightarrow> bool"
   fp32_from_int :: "ieee_rounding \<Rightarrow> int \<Rightarrow> 32 word"
   fp32_greater :: "32 word \<Rightarrow> 32 word \<Rightarrow> bool"
   fp32_greater_equal :: "32 word \<Rightarrow> 32 word \<Rightarrow> bool"
+  fp32_is_integral :: "32 word \<Rightarrow> bool"
   fp32_is_finite :: "32 word \<Rightarrow> bool"
   fp32_is_nan :: "32 word \<Rightarrow> bool"
   fp32_is_normal :: "32 word \<Rightarrow> bool"
+  fp32_is_signalling_nan :: "32 word \<Rightarrow> bool"
   fp32_is_subnormal :: "32 word \<Rightarrow> bool"
   fp32_less :: "32 word \<Rightarrow> 32 word \<Rightarrow> bool"
   fp32_less_equal :: "32 word \<Rightarrow> 32 word \<Rightarrow> bool"
   fp32_mul :: "ieee_rounding \<Rightarrow> 32 word \<Rightarrow> 32 word \<Rightarrow> 32 word"
+  fp32_mul_with_flags :: "ieee_rounding \<Rightarrow> 32 word \<Rightarrow> 32 word \<Rightarrow> ieee_flags \<times> 32 word"
   fp32_mul_add :: "ieee_rounding \<Rightarrow> 32 word \<Rightarrow> 32 word \<Rightarrow> 32 word \<Rightarrow> 32 word"
+  fp32_mul_add_with_flags :: "ieee_rounding \<Rightarrow> 32 word \<Rightarrow> 32 word \<Rightarrow> 32 word \<Rightarrow> ieee_flags \<times> 32 word"
   fp32_mul_sub :: "ieee_rounding \<Rightarrow> 32 word \<Rightarrow> 32 word \<Rightarrow> 32 word \<Rightarrow> 32 word"
+  fp32_mul_sub_with_flags :: "ieee_rounding \<Rightarrow> 32 word \<Rightarrow> 32 word \<Rightarrow> 32 word \<Rightarrow> ieee_flags \<times> 32 word"
   fp32_neg_inf :: "32 word"
+  fp32_neg_max :: "32 word"
+  fp32_neg_min :: "32 word"
   fp32_neg_zero :: "32 word"
   fp32_negate :: "32 word \<Rightarrow> 32 word"
-  fp32_negate1985 :: "32 word \<Rightarrow> 32 word"
   fp32_pos_inf :: "32 word"
+  fp32_pos_max :: "32 word"
+  fp32_pos_min :: "32 word"
   fp32_pos_zero :: "32 word"
+  fp32_round_to_integral :: "ieee_rounding \<Rightarrow> 32 word \<Rightarrow> 32 word"
+  fp32_snan :: "32 word"
   fp32_sqrt :: "ieee_rounding \<Rightarrow> 32 word \<Rightarrow> 32 word"
+  fp32_sqrt_with_flags :: "ieee_rounding \<Rightarrow> 32 word \<Rightarrow> ieee_flags \<times> 32 word"
   fp32_sub :: "ieee_rounding \<Rightarrow> 32 word \<Rightarrow> 32 word \<Rightarrow> 32 word"
+  fp32_sub_with_flags :: "ieee_rounding \<Rightarrow> 32 word \<Rightarrow> 32 word \<Rightarrow> ieee_flags \<times> 32 word"
+  fp32_qnan :: "32 word"
   fp32_to_int :: "ieee_rounding \<Rightarrow> 32 word \<Rightarrow> int option"
 
 consts
   fp64_abs :: "64 word \<Rightarrow> 64 word"
-  fp64_abs1985 :: "64 word \<Rightarrow> 64 word"
   fp64_add :: "ieee_rounding \<Rightarrow> 64 word \<Rightarrow> 64 word \<Rightarrow> 64 word"
+  fp64_add_with_flags :: "ieee_rounding \<Rightarrow> 64 word \<Rightarrow> 64 word \<Rightarrow> ieee_flags \<times> 64 word"
   fp64_compare :: "64 word \<Rightarrow> 64 word \<Rightarrow> ieee_compare"
   fp64_div :: "ieee_rounding \<Rightarrow> 64 word \<Rightarrow> 64 word \<Rightarrow> 64 word"
+  fp64_div_with_flags :: "ieee_rounding \<Rightarrow> 64 word \<Rightarrow> 64 word \<Rightarrow> ieee_flags \<times> 64 word"
   fp64_equal :: "64 word \<Rightarrow> 64 word \<Rightarrow> bool"
   fp64_from_int :: "ieee_rounding \<Rightarrow> int \<Rightarrow> 64 word"
   fp64_greater :: "64 word \<Rightarrow> 64 word \<Rightarrow> bool"
   fp64_greater_equal :: "64 word \<Rightarrow> 64 word \<Rightarrow> bool"
+  fp64_is_integral :: "64 word \<Rightarrow> bool"
   fp64_is_finite :: "64 word \<Rightarrow> bool"
   fp64_is_nan :: "64 word \<Rightarrow> bool"
   fp64_is_normal :: "64 word \<Rightarrow> bool"
+  fp64_is_signalling_nan :: "64 word \<Rightarrow> bool"
   fp64_is_subnormal :: "64 word \<Rightarrow> bool"
   fp64_less :: "64 word \<Rightarrow> 64 word \<Rightarrow> bool"
   fp64_less_equal :: "64 word \<Rightarrow> 64 word \<Rightarrow> bool"
   fp64_mul :: "ieee_rounding \<Rightarrow> 64 word \<Rightarrow> 64 word \<Rightarrow> 64 word"
+  fp64_mul_with_flags :: "ieee_rounding \<Rightarrow> 64 word \<Rightarrow> 64 word \<Rightarrow> ieee_flags \<times> 64 word"
   fp64_mul_add :: "ieee_rounding \<Rightarrow> 64 word \<Rightarrow> 64 word \<Rightarrow> 64 word \<Rightarrow> 64 word"
+  fp64_mul_add_with_flags :: "ieee_rounding \<Rightarrow> 64 word \<Rightarrow> 64 word \<Rightarrow> 64 word \<Rightarrow> ieee_flags \<times> 64 word"
   fp64_mul_sub :: "ieee_rounding \<Rightarrow> 64 word \<Rightarrow> 64 word \<Rightarrow> 64 word \<Rightarrow> 64 word"
+  fp64_mul_sub_with_flags :: "ieee_rounding \<Rightarrow> 64 word \<Rightarrow> 64 word \<Rightarrow> 64 word \<Rightarrow> ieee_flags \<times> 64 word"
   fp64_neg_inf :: "64 word"
+  fp64_neg_min :: "64 word"
+  fp64_neg_max :: "64 word"
   fp64_neg_zero :: "64 word"
   fp64_negate :: "64 word \<Rightarrow> 64 word"
-  fp64_negate1985 :: "64 word \<Rightarrow> 64 word"
   fp64_pos_inf :: "64 word"
+  fp64_pos_min :: "64 word"
+  fp64_pos_max :: "64 word"
   fp64_pos_zero :: "64 word"
+  fp64_round_to_integral :: "ieee_rounding \<Rightarrow> 64 word \<Rightarrow> 64 word"
+  fp64_snan :: "64 word"
   fp64_sqrt :: "ieee_rounding \<Rightarrow> 64 word \<Rightarrow> 64 word"
+  fp64_sqrt_with_flags :: "ieee_rounding \<Rightarrow> 64 word \<Rightarrow> ieee_flags \<times> 64 word"
   fp64_sub :: "ieee_rounding \<Rightarrow> 64 word \<Rightarrow> 64 word \<Rightarrow> 64 word"
+  fp64_sub_with_flags :: "ieee_rounding \<Rightarrow> 64 word \<Rightarrow> 64 word \<Rightarrow> ieee_flags \<times> 64 word"
+  fp64_qnan :: "64 word"
   fp64_to_int :: "ieee_rounding \<Rightarrow> 64 word \<Rightarrow> int option"
 
 consts
@@ -433,14 +659,14 @@ code_printing
       (SML) "!(fn '_ => raise Fail \"fp32'_abs\")"
       and (OCaml) "!(fun '_ -> failwith \"fp32'_abs\")"
       and (Haskell) "!(\\ '_ -> error \"fp32'_abs\")"
-  | constant "fp32_abs1985" \<rightharpoonup>
-      (SML) "!(fn '_ => raise Fail \"fp32'_abs1985\")"
-      and (OCaml) "!(fun '_ -> failwith \"fp32'_abs1985\")"
-      and (Haskell) "!(\\ '_ -> error \"fp32'_abs1985\")"
   | constant "fp32_add" \<rightharpoonup>
       (SML) "!(fn '_ => fn '_ => fn '_ => raise Fail \"fp32'_add\")"
       and (OCaml) "!(fun '_ '_ '_ -> failwith \"fp32'_add\")"
       and (Haskell) "!(\\ '_ '_ '_ -> error \"fp32'_add\")"
+  | constant "fp32_add_with_flags" \<rightharpoonup>
+      (SML) "!(fn '_ => fn '_ => fn '_ => raise Fail \"fp32'_add'_with'_flags\")"
+      and (OCaml) "!(fun '_ '_ '_ -> failwith \"fp32'_add'_with'_flag\")"
+      and (Haskell) "!(\\ '_ '_ '_ -> error \"fp32'_add'_with'_flag\")"
   | constant "fp32_compare" \<rightharpoonup>
       (SML) "!(fn '_ => fn '_ => raise Fail \"fp32'_compare\")"
       and (OCaml) "!(fun '_ '_ -> failwith \"fp32'_compare\")"
@@ -449,6 +675,10 @@ code_printing
       (SML) "!(fn '_ => fn '_ => fn '_ => raise Fail \"fp32'_div\")"
       and (OCaml) "!(fun '_ '_ '_ -> failwith \"fp32'_div\")"
       and (Haskell) "!(\\ '_ '_ '_ -> error \"fp32'_div\")"
+  | constant "fp32_div_with_flags" \<rightharpoonup>
+      (SML) "!(fn '_ => fn '_ => fn '_ => raise Fail \"fp32'_div'_with'_flags\")"
+      and (OCaml) "!(fun '_ '_ '_ -> failwith \"fp32'_div'_with'_flag\")"
+      and (Haskell) "!(\\ '_ '_ '_ -> error \"fp32'_div'_with'_flag\")"
   | constant "fp32_equal" \<rightharpoonup>
       (SML) "!(fn '_ => fn '_ => raise Fail \"fp32'_equal\")"
       and (OCaml) "!(fun '_ '_ -> failwith \"fp32'_equal\")"
@@ -465,6 +695,10 @@ code_printing
       (SML) "!(fn '_ => fn '_ => raise Fail \"fp32'_greater'_equal\")"
       and (OCaml) "!(fun '_ '_ -> failwith \"fp32'_greater'_equal\")"
       and (Haskell) "!(\\ '_ '_ -> error \"fp32'_greater'_equal\")"
+  | constant "fp32_is_integral" \<rightharpoonup>
+      (SML) "!(fn '_ => raise Fail \"fp32'_is'_integral\")"
+      and (OCaml) "!(fun '_ -> failwith \"fp32'_is'_integral\")"
+      and (Haskell) "!(\\ '_ -> error \"fp32'_is'_intagral\")"
   | constant "fp32_is_finite" \<rightharpoonup>
       (SML) "!(fn '_ => raise Fail \"fp32'_is'_finite\")"
       and (OCaml) "!(fun '_ -> failwith \"fp32'_is'_finite\")"
@@ -477,6 +711,10 @@ code_printing
       (SML) "!(fn '_ => raise Fail \"fp32'_is'_normal\")"
       and (OCaml) "!(fun '_ -> failwith \"fp32'_is'_normal\")"
       and (Haskell) "!(\\ '_ -> error \"fp32'_is'_normal\")"
+  | constant "fp32_is_signalling_nan" \<rightharpoonup>
+      (SML) "!(fn '_ => raise Fail \"fp32'_is'_signalling'_nan\")"
+      and (OCaml) "!(fun '_ -> failwith \"fp32'_is'_signalling'_nan\")"
+      and (Haskell) "!(\\ '_ -> error \"fp32'_is'_signalling'_nan\")"
   | constant "fp32_is_subnormal" \<rightharpoonup>
       (SML) "!(fn '_ => raise Fail \"fp32'_is'_subnormal\")"
       and (OCaml) "!(fun '_ -> failwith \"fp32'_is'_subnormal\")"
@@ -493,18 +731,38 @@ code_printing
       (SML) "!(fn '_ => fn '_ => fn '_ => raise Fail \"fp32'_mul\")"
       and (OCaml) "!(fun '_ '_ '_ -> failwith \"fp32'_mul\")"
       and (Haskell) "!(\\ '_ '_ '_ -> error \"fp32'_mul\")"
+  | constant "fp32_mul_with_flags" \<rightharpoonup>
+      (SML) "!(fn '_ => fn '_ => fn '_ => raise Fail \"fp32'_mul'_with'_flags\")"
+      and (OCaml) "!(fun '_ '_ '_ -> failwith \"fp32'_mul'_with'_flag\")"
+      and (Haskell) "!(\\ '_ '_ '_ -> error \"fp32'_mul'_with'_flag\")"
   | constant "fp32_mul_add" \<rightharpoonup>
       (SML) "!(fn '_ => fn '_ => fn '_ => fn '_ => raise Fail \"fp32'_mul'_add\")"
       and (OCaml) "!(fun '_ '_ '_ '_ -> failwith \"fp32'_mul'_add\")"
       and (Haskell) "!(\\ '_ '_ '_ '_ -> error \"fp32'_mul'_add\")"
+  | constant "fp32_mul_add_with_flags" \<rightharpoonup>
+      (SML) "!(fn '_ => fn '_ => fn '_ => raise Fail \"fp32'_mul'_add'_with'_flags\")"
+      and (OCaml) "!(fun '_ '_ '_ -> failwith \"fp32'_mul'_add'_with'_flag\")"
+      and (Haskell) "!(\\ '_ '_ '_ -> error \"fp32'_mul'_add'_with'_flag\")"
   | constant "fp32_mul_sub" \<rightharpoonup>
       (SML) "!(fn '_ => fn '_ => fn '_ => fn '_ => raise Fail \"fp32'_mul'_sub\")"
       and (OCaml) "!(fun '_ '_ '_ '_ -> failwith \"fp32'_mul'_sub\")"
       and (Haskell) "!(\\ '_ '_ '_ '_ -> error \"fp32'_mul'_sub\")"
+  | constant "fp32_mul_sub_with_flags" \<rightharpoonup>
+      (SML) "!(fn '_ => fn '_ => fn '_ => raise Fail \"fp32'_sub'_add'_with'_flags\")"
+      and (OCaml) "!(fun '_ '_ '_ -> failwith \"fp32'_mul'_sub'_with'_flag\")"
+      and (Haskell) "!(\\ '_ '_ '_ -> error \"fp32'_mul'_sub'_with'_flag\")"
   | constant "fp32_neg_inf" \<rightharpoonup>
       (SML) "!(raise Fail \"fp32'_neg'_inf\")"
       and (OCaml) "!(failwith \"fp32'_neg'_inf\")"
       and (Haskell) "!(error \"fp32'_neg'_inf\")"
+  | constant "fp32_neg_min" \<rightharpoonup>
+      (SML) "!(raise Fail \"fp32'_neg'_min\")"
+      and (OCaml) "!(failwith \"fp32'_neg'_min\")"
+      and (Haskell) "!(error \"fp32'_neg'_min\")"
+  | constant "fp32_neg_max" \<rightharpoonup>
+      (SML) "!(raise Fail \"fp32'_neg'_max\")"
+      and (OCaml) "!(failwith \"fp32'_neg'_max\")"
+      and (Haskell) "!(error \"fp32'_neg'_min\")"
   | constant "fp32_neg_zero" \<rightharpoonup>
       (SML) "!(raise Fail \"fp32'_neg'_zero\")"
       and (OCaml) "!(failwith \"fp32'_neg'_zero\")"
@@ -513,26 +771,50 @@ code_printing
       (SML) "!(fn '_ => raise Fail \"fp32'_negate\")"
       and (OCaml) "!(fun '_ -> failwith \"fp32'_negate\")"
       and (Haskell) "!(\\ '_ -> error \"fp32'_negate\")"
-  | constant "fp32_negate1985" \<rightharpoonup>
-      (SML) "!(fn '_ => raise Fail \"fp32'_negate1985\")"
-      and (OCaml) "!(fun '_ -> failwith \"fp32'_negate1985\")"
-      and (Haskell) "!(\\ '_ -> error \"fp32'_negate1985\")"
   | constant "fp32_pos_inf" \<rightharpoonup>
       (SML) "!(raise Fail \"fp32'_pos'_inf\")"
       and (OCaml) "!(failwith \"fp32'_pos'_inf\")"
       and (Haskell) "!(error \"fp32'_pos'_inf\")"
+  | constant "fp32_pos_min" \<rightharpoonup>
+      (SML) "!(raise Fail \"fp32'_pos'_min\")"
+      and (OCaml) "!(failwith \"fp32'_pos'_min\")"
+      and (Haskell) "!(error \"fp32'_pos'_min\")"
+  | constant "fp32_pos_max" \<rightharpoonup>
+      (SML) "!(raise Fail \"fp32'_pos'_max\")"
+      and (OCaml) "!(failwith \"fp32'_pos'_max\")"
+      and (Haskell) "!(error \"fp32'_pos'_max\")"
   | constant "fp32_pos_zero" \<rightharpoonup>
       (SML) "!(raise Fail \"fp32'_pos'_zero\")"
       and (OCaml) "!(failwith \"fp32'_pos'_zero\")"
       and (Haskell) "!(error \"fp32'_pos'_zero\")"
+  | constant "fp32_snan" \<rightharpoonup>
+      (SML) "!(raise Fail \"fp32'_snan\")"
+      and (OCaml) "!(failwith \"fp32'_snan\")"
+      and (Haskell) "!(error \"fp32'_snan\")"
+  | constant "fp32_round_to_integral" \<rightharpoonup>
+      (SML) "!(fn '_ => fn '_ => raise Fail \"fp32'_round'_to'_integral\")"
+      and (OCaml) "!(fun '_ '_ -> failwith \"fp32'_round'_to'_integral\")"
+      and (Haskell) "!(\\ '_ '_ -> error \"fp32'_to'_integral\")"
   | constant "fp32_sqrt" \<rightharpoonup>
       (SML) "!(fn '_ => fn '_ => raise Fail \"fp32'_sqrt\")"
       and (OCaml) "!(fun '_ '_ -> failwith \"fp32'_sqrt\")"
       and (Haskell) "!(\\ '_ '_ -> error \"fp32'_sqrt\")"
+  | constant "fp32_sqrt_with_flags" \<rightharpoonup>
+      (SML) "!(fn '_ => fn '_ => fn '_ => raise Fail \"fp32'_sqrt'_with'_flags\")"
+      and (OCaml) "!(fun '_ '_ '_ -> failwith \"fp32'_sqrt'_with'_flag\")"
+      and (Haskell) "!(\\ '_ '_ '_ -> error \"fp32'_sqrt'_with'_flag\")"
   | constant "fp32_sub" \<rightharpoonup>
       (SML) "!(fn '_ => fn '_ => fn '_ => raise Fail \"fp32'_sub\")"
       and (OCaml) "!(fun '_ '_ '_ -> failwith \"fp32'_sub\")"
       and (Haskell) "!(\\ '_ '_ '_ -> error \"fp32'_sub\")"
+  | constant "fp32_sub_with_flags" \<rightharpoonup>
+      (SML) "!(fn '_ => fn '_ => fn '_ => raise Fail \"fp32'_sub'_with'_flags\")"
+      and (OCaml) "!(fun '_ '_ '_ -> failwith \"fp32'_sub'_with'_flag\")"
+      and (Haskell) "!(\\ '_ '_ '_ -> error \"fp32'_sub'_with'_flag\")"
+  | constant "fp32_qnan" \<rightharpoonup>
+      (SML) "!(raise Fail \"fp32'_qnan\")"
+      and (OCaml) "!(failwith \"fp32'_qnan\")"
+      and (Haskell) "!(error \"fp32'_qnan\")"
   | constant "fp32_to_int" \<rightharpoonup>
       (SML) "!(fn '_ => fn '_ => raise Fail \"fp32'_to'_int\")"
       and (OCaml) "!(fun '_ '_ -> failwith \"fp32'_to'_int\")"
@@ -541,14 +823,14 @@ code_printing
       (SML) "!(fn '_ => raise Fail \"fp64'_abs\")"
       and (OCaml) "!(fun '_ -> failwith \"fp64'_abs\")"
       and (Haskell) "!(\\ '_ -> error \"fp64'_abs\")"
-  | constant "fp64_abs1985" \<rightharpoonup>
-      (SML) "!(fn '_ => raise Fail \"fp64'_abs1985\")"
-      and (OCaml) "!(fun '_ -> failwith \"fp64'_abs1985\")"
-      and (Haskell) "!(\\ '_ -> error \"fp64'_abs1985\")"
   | constant "fp64_add" \<rightharpoonup>
       (SML) "!(fn '_ => fn '_ => fn '_ => raise Fail \"fp64'_add\")"
       and (OCaml) "!(fun '_ '_ '_ -> failwith \"fp64'_add\")"
       and (Haskell) "!(\\ '_ '_ '_ -> error \"fp64'_add\")"
+  | constant "fp64_add_with_flags" \<rightharpoonup>
+      (SML) "!(fn '_ => fn '_ => fn '_ => raise Fail \"fp64'_add'_with'_flags\")"
+      and (OCaml) "!(fun '_ '_ '_ -> failwith \"fp64'_add'_with'_flag\")"
+      and (Haskell) "!(\\ '_ '_ '_ -> error \"fp64'_add'_with'_flag\")"
   | constant "fp64_compare" \<rightharpoonup>
       (SML) "!(fn '_ => fn '_ => raise Fail \"fp64'_compare\")"
       and (OCaml) "!(fun '_ '_ -> failwith \"fp64'_compare\")"
@@ -557,6 +839,10 @@ code_printing
       (SML) "!(fn '_ => fn '_ => fn '_ => raise Fail \"fp64'_div\")"
       and (OCaml) "!(fun '_ '_ '_ -> failwith \"fp64'_div\")"
       and (Haskell) "!(\\ '_ '_ '_ -> error \"fp64'_div\")"
+  | constant "fp64_div_with_flags" \<rightharpoonup>
+      (SML) "!(fn '_ => fn '_ => fn '_ => raise Fail \"fp64'_div'_with'_flags\")"
+      and (OCaml) "!(fun '_ '_ '_ -> failwith \"fp64'_div'_with'_flag\")"
+      and (Haskell) "!(\\ '_ '_ '_ -> error \"fp64'_div'_with'_flag\")"
   | constant "fp64_equal" \<rightharpoonup>
       (SML) "!(fn '_ => fn '_ => raise Fail \"fp64'_equal\")"
       and (OCaml) "!(fun '_ '_ -> failwith \"fp64'_equal\")"
@@ -573,6 +859,10 @@ code_printing
       (SML) "!(fn '_ => fn '_ => raise Fail \"fp64'_greater'_equal\")"
       and (OCaml) "!(fun '_ '_ -> failwith \"fp64'_greater'_equal\")"
       and (Haskell) "!(\\ '_ '_ -> error \"fp64'_greater'_equal\")"
+  | constant "fp64_is_integral" \<rightharpoonup>
+      (SML) "!(fn '_ => raise Fail \"fp64'_is'_integral\")"
+      and (OCaml) "!(fun '_ -> failwith \"fp64'_is'_integral\")"
+      and (Haskell) "!(\\ '_ -> error \"fp64'_is'_intagral\")"
   | constant "fp64_is_finite" \<rightharpoonup>
       (SML) "!(fn '_ => raise Fail \"fp64'_is'_finite\")"
       and (OCaml) "!(fun '_ -> failwith \"fp64'_is'_finite\")"
@@ -585,6 +875,10 @@ code_printing
       (SML) "!(fn '_ => raise Fail \"fp64'_is'_normal\")"
       and (OCaml) "!(fun '_ -> failwith \"fp64'_is'_normal\")"
       and (Haskell) "!(\\ '_ -> error \"fp64'_is'_normal\")"
+  | constant "fp64_is_signalling_nan" \<rightharpoonup>
+      (SML) "!(fn '_ => raise Fail \"fp64'_is'_signalling'_nan\")"
+      and (OCaml) "!(fun '_ -> failwith \"fp64'_is'_signalling'_nan\")"
+      and (Haskell) "!(\\ '_ -> error \"fp64'_is'_signalling'_nan\")"
   | constant "fp64_is_subnormal" \<rightharpoonup>
       (SML) "!(fn '_ => raise Fail \"fp64'_is'_subnormal\")"
       and (OCaml) "!(fun '_ -> failwith \"fp64'_is'_subnormal\")"
@@ -601,18 +895,38 @@ code_printing
       (SML) "!(fn '_ => fn '_ => fn '_ => raise Fail \"fp64'_mul\")"
       and (OCaml) "!(fun '_ '_ '_ -> failwith \"fp64'_mul\")"
       and (Haskell) "!(\\ '_ '_ '_ -> error \"fp64'_mul\")"
+  | constant "fp64_mul_with_flags" \<rightharpoonup>
+      (SML) "!(fn '_ => fn '_ => fn '_ => raise Fail \"fp64'_mul'_with'_flags\")"
+      and (OCaml) "!(fun '_ '_ '_ -> failwith \"fp64'_mul'_with'_flag\")"
+      and (Haskell) "!(\\ '_ '_ '_ -> error \"fp64'_mul'_with'_flag\")"
   | constant "fp64_mul_add" \<rightharpoonup>
       (SML) "!(fn '_ => fn '_ => fn '_ => fn '_ => raise Fail \"fp64'_mul'_add\")"
       and (OCaml) "!(fun '_ '_ '_ '_ -> failwith \"fp64'_mul'_add\")"
       and (Haskell) "!(\\ '_ '_ '_ '_ -> error \"fp64'_mul'_add\")"
+  | constant "fp64_mul_add_with_flags" \<rightharpoonup>
+      (SML) "!(fn '_ => fn '_ => fn '_ => raise Fail \"fp64'_mul'_add'_with'_flags\")"
+      and (OCaml) "!(fun '_ '_ '_ -> failwith \"fp64'_mul'_add'_with'_flag\")"
+      and (Haskell) "!(\\ '_ '_ '_ -> error \"fp64'_mul'_add'_with'_flag\")"
   | constant "fp64_mul_sub" \<rightharpoonup>
       (SML) "!(fn '_ => fn '_ => fn '_ => fn '_ => raise Fail \"fp64'_mul'_sub\")"
       and (OCaml) "!(fun '_ '_ '_ '_ -> failwith \"fp64'_mul'_sub\")"
       and (Haskell) "!(\\ '_ '_ '_ '_ -> error \"fp64'_mul'_sub\")"
+  | constant "fp64_mul_sub_with_flags" \<rightharpoonup>
+      (SML) "!(fn '_ => fn '_ => fn '_ => raise Fail \"fp64'_sub'_add'_with'_flags\")"
+      and (OCaml) "!(fun '_ '_ '_ -> failwith \"fp64'_mul'_sub'_with'_flag\")"
+      and (Haskell) "!(\\ '_ '_ '_ -> error \"fp64'_mul'_sub'_with'_flag\")"
   | constant "fp64_neg_inf" \<rightharpoonup>
       (SML) "!(raise Fail \"fp64'_neg'_inf\")"
       and (OCaml) "!(failwith \"fp64'_neg'_inf\")"
       and (Haskell) "!(error \"fp64'_neg'_inf\")"
+  | constant "fp64_neg_min" \<rightharpoonup>
+      (SML) "!(raise Fail \"fp64'_neg'_min\")"
+      and (OCaml) "!(failwith \"fp64'_neg'_min\")"
+      and (Haskell) "!(error \"fp64'_neg'_min\")"
+  | constant "fp64_neg_max" \<rightharpoonup>
+      (SML) "!(raise Fail \"fp64'_neg'_max\")"
+      and (OCaml) "!(failwith \"fp64'_neg'_max\")"
+      and (Haskell) "!(error \"fp64'_neg'_max\")"
   | constant "fp64_neg_zero" \<rightharpoonup>
       (SML) "!(raise Fail \"fp64'_neg'_zero\")"
       and (OCaml) "!(failwith \"fp64'_neg'_zero\")"
@@ -621,26 +935,50 @@ code_printing
       (SML) "!(fn '_ => raise Fail \"fp64'_negate\")"
       and (OCaml) "!(fun '_ -> failwith \"fp64'_negate\")"
       and (Haskell) "!(\\ '_ -> error \"fp64'_negate\")"
-  | constant "fp64_negate1985" \<rightharpoonup>
-      (SML) "!(fn '_ => raise Fail \"fp64'_negate1985\")"
-      and (OCaml) "!(fun '_ -> failwith \"fp64'_negate1985\")"
-      and (Haskell) "!(\\ '_ -> error \"fp64'_negate1985\")"
   | constant "fp64_pos_inf" \<rightharpoonup>
       (SML) "!(raise Fail \"fp64'_pos'_inf\")"
       and (OCaml) "!(failwith \"fp64'_pos'_inf\")"
       and (Haskell) "!(error \"fp64'_pos'_inf\")"
+  | constant "fp64_pos_min" \<rightharpoonup>
+      (SML) "!(raise Fail \"fp64'_pos'_min\")"
+      and (OCaml) "!(failwith \"fp64'_pos'_min\")"
+      and (Haskell) "!(error \"fp64'_pos'_min\")"
+  | constant "fp64_pos_max" \<rightharpoonup>
+      (SML) "!(raise Fail \"fp64'_pos'_max\")"
+      and (OCaml) "!(failwith \"fp64'_pos'_max\")"
+      and (Haskell) "!(error \"fp64'_pos'_max\")"
   | constant "fp64_pos_zero" \<rightharpoonup>
       (SML) "!(raise Fail \"fp64'_pos'_zero\")"
       and (OCaml) "!(failwith \"fp64'_pos'_zero\")"
       and (Haskell) "!(error \"fp64'_pos'_zero\")"
+  | constant "fp64_snan" \<rightharpoonup>
+      (SML) "!(raise Fail \"fp64'_snan\")"
+      and (OCaml) "!(failwith \"fp64'_snan\")"
+      and (Haskell) "!(error \"fp64'_snan\")"
+  | constant "fp64_round_to_integral" \<rightharpoonup>
+      (SML) "!(fn '_ => fn '_ => raise Fail \"fp64'_round'_to'_integral\")"
+      and (OCaml) "!(fun '_ '_ -> failwith \"fp64'_round'_to'_integral\")"
+      and (Haskell) "!(\\ '_ '_ -> error \"fp64'_to'_integral\")"
   | constant "fp64_sqrt" \<rightharpoonup>
       (SML) "!(fn '_ => fn '_ => raise Fail \"fp64'_sqrt\")"
       and (OCaml) "!(fun '_ '_ -> failwith \"fp64'_sqrt\")"
       and (Haskell) "!(\\ '_ '_ -> error \"fp64'_sqrt\")"
+  | constant "fp64_sqrt_with_flags" \<rightharpoonup>
+      (SML) "!(fn '_ => fn '_ => fn '_ => raise Fail \"fp64'_sqrt'_with'_flags\")"
+      and (OCaml) "!(fun '_ '_ '_ -> failwith \"fp64'_sqrt'_with'_flag\")"
+      and (Haskell) "!(\\ '_ '_ '_ -> error \"fp64'_sqrt'_with'_flag\")"
+  | constant "fp64_qnan" \<rightharpoonup>
+      (SML) "!(raise Fail \"fp64'_qnan\")"
+      and (OCaml) "!(failwith \"fp64'_qnan\")"
+      and (Haskell) "!(error \"fp64'_qnan\")"
   | constant "fp64_sub" \<rightharpoonup>
       (SML) "!(fn '_ => fn '_ => fn '_ => raise Fail \"fp64'_sub\")"
       and (OCaml) "!(fun '_ '_ '_ -> failwith \"fp64'_sub\")"
       and (Haskell) "!(\\ '_ '_ '_ -> error \"fp64'_sub\")"
+  | constant "fp64_sub_with_flags" \<rightharpoonup>
+      (SML) "!(fn '_ => fn '_ => fn '_ => raise Fail \"fp64'_sub'_with'_flags\")"
+      and (OCaml) "!(fun '_ '_ '_ -> failwith \"fp64'_sub'_with'_flag\")"
+      and (Haskell) "!(\\ '_ '_ '_ -> error \"fp64'_sub'_with'_flag\")"
   | constant "fp64_to_int" \<rightharpoonup>
       (SML) "!(fn '_ => fn '_ => raise Fail \"fp64'_to'_int\")"
       and (OCaml) "!(fun '_ '_ -> failwith \"fp64'_to'_int\")"
